Semantic/Stlc/Substitution.lean
@@ -1,4 +1,5 @@
 import Semantic.Stlc.Syntax
+import Mathlib.Tactic
 
 structure Subst (n1 n2 : Nat) where
   exp : Var n1 -> Exp n2
@@ -8,7 +9,12 @@ def Subst.liftVar (s : Subst n1 n2) : Subst (n1+1) (n2+1) where
     | .here => .var .here
     | .there x => (s.exp x).rename Rename.succVar
 
-def Subst.id (n : Nat) : Subst n n where
+def Subst.lift (s : Subst n1 n2) (k : Nat) : Subst (n1+k) (n2+k) :=
+  match k with
+  | 0 => s
+  | k+1 => (s.lift k).liftVar
+
+def Subst.id : Subst n n where
   exp := fun x => .var x
 
 def Subst.openVar (e : Exp n) : Subst (n+1) n where
@@ -53,3 +59,53 @@ theorem Exp.subst_IsVal {e : Exp n1} {s : Subst n1 n2}
 def Val.subst {n1 n2 : Nat} (v : Val n1) (s : Subst n1 n2) : Val n2 where
   unwrap := v.unwrap.subst s
   isVal := Exp.subst_IsVal v.isVal
+
+theorem Subst.funext {s1 s2 : Subst n1 n2}
+  (exp : ∀ x, s1.exp x = s2.exp x) :
+  s1 = s2 := by
+  cases s1; cases s2
+  aesop
+
+theorem Subst.id_liftVar {n : Nat} :
+  (Subst.id (n:=n)).liftVar = Subst.id := by
+  apply Subst.funext
+  intro x
+  cases x <;> rfl
+
+theorem Exp.subst_id {e : Exp n} :
+  e.subst Subst.id = e := by
+  induction e <;> try grind [Exp.subst, Subst.id]
+  case var => rfl
+  case abs ih => simpa [Exp.subst, Subst.id_liftVar]
+
+def Subst.comp (s1 : Subst n1 n2) (s2 : Subst n2 n3) : Subst n1 n3 where
+  exp := fun x => (s1.exp x).subst s2
+
+theorem Exp.weaken_subst_comm {e : Exp (n1 + k)} {s : Subst n1 n2} :
+  (e.subst (s.lift k)).rename (Rename.succVar.lift k) =
+    (e.rename (Rename.succVar.lift k)).subst (s.liftVar.lift k) := by
+  sorry
+
+theorem Subst.comp_liftVar {s1 : Subst n1 n2} {s2 : Subst n2 n3} :
+  (s1.liftVar).comp (s2.liftVar) = (s1.comp s2).liftVar := by
+  apply Subst.funext
+  intro x
+  cases x
+  case here => rfl
+  case there x =>
+    conv => rhs; simp [Subst.liftVar, Subst.comp]
+    conv =>
+      lhs
+      simp [Subst.comp]
+      arg 1
+      simp [Subst.liftVar]
+    sorry
+
+theorem Exp.subst_comp {e : Exp n1} {s1 : Subst n1 n2} {s2 : Subst n2 n3} :
+  (e.subst s1).subst s2 = e.subst (s1.comp s2) := by
+  induction e generalizing n2 n3 <;> try grind [Exp.subst, Subst.comp]
+  case var => rfl
+  case abs ih =>
+    simp [Exp.subst]
+    convert ih
+    sorry
