Semantic/Stlc/RebindTheory.lean
@@ -8,34 +8,24 @@ structure Rebind (s1 : Store n1) (f : Rename n1 n2) (s2 : Store n2) where
   var : ∀ (x : Var n1),
     s2.lookup (f.var x) = (s1.lookup x).rename f
 
-theorem eval_rebind {f : Rename n1 n2}
-  (ρ : Rebind s1 f s2)
-  (e : Exp n1) :
-  eval s2 (e.rename f) fuel = (eval s1 e fuel).rename f := by
-  induction e generalizing fuel s2
-  case var x0 =>
-    cases fuel
-    case zero => rfl
-    case succ fuel =>
-      simp [Exp.rename, eval]
-      have := ρ.var x0
-      grind [EvalResult.rename]
-  case abs ih =>
-    cases fuel
-    case zero => rfl
-    case succ fuel =>
-      simp [Exp.rename, eval]
-      grind [EvalResult.rename, Exp.rename]
-  case app ih1 ih2 =>
-    cases fuel
-    case zero => rfl
-    case succ fuel =>
-      conv => lhs; simp [Exp.rename]
-      sorry
-  case btrue => sorry
-  case bfalse => sorry
-  case nzero => sorry
-  case nsucc => sorry
-  case pred => sorry
-  case iszero => sorry
-  case cond => sorry
+def Eval.rebind {f : Rename n1 n2}
+  (hev : Eval s1 e1 v1)
+  (ρ : Rebind s1 f s2) :
+  Eval s2 (e1.rename f) (v1.rename f) := by
+  induction hev generalizing n2
+  case ev_var x0 =>
+    have h := ρ.var x0
+    simp [<-h]
+    grind [Exp.rename, Eval]
+  case ev_app ih1 ih2 => sorry
+  case ev_abs => sorry
+  case ev_nsucc ih => sorry
+  case ev_btrue => sorry
+  case ev_bfalse => sorry
+  case ev_nzero => sorry
+  case ev_pred_nzero ih => sorry
+  case ev_pred_nsucc ih => sorry
+  case ev_iszero_nzero ih => sorry
+  case ev_iszero_nsucc ih => sorry
+  case ev_cond_true ih1 ih2 => sorry
+  case ev_cond_false ih1 ih2 => sorry
